3.3. talks abiyt conversion. More todos, a fix to fig 3, new file for dependent prolog tactic

tactics/prolog.v
@@ -1,13 +1,15 @@
-(*"prolog"-like tactic modulo FPC for height, size and pairing thereof  -- am*)
+(* NON dependent "prolog"-like tactic modulo FPC for height, size and pairing thereof
+
+OBSOLETE: go to dprolog.v*)
 
 From elpi Require Import elpi.
 Require Import Arith List. Import ListNotations.
 Require Import Coq.Lists.List.
 
 Elpi Tactic prolog.
-Elpi Accumulate File "pbt/src/kernel.mod".
-Elpi Accumulate File "pbt/src/fpc-qbound.mod".
-Elpi Accumulate File "pbt/src/fpc-pair.mod".
+Elpi Accumulate File "pbt/kernel.mod".
+Elpi Accumulate File "pbt/fpc-qbound.mod".
+Elpi Accumulate File "pbt/fpc-pair.mod".
 
 
 Elpi Accumulate lp:{{
@@ -27,30 +29,9 @@ Elpi Accumulate lp:{{
   }}. 
 Elpi Typecheck.
 
-Elpi Tactic dprolog.
-Elpi Accumulate File "pbt/src/dep-kernel.mod".
-Elpi Accumulate File "pbt/src/fpc-qbound.mod".
-Elpi Accumulate File "pbt/src/fpc-pair.mod".
 
-Elpi Accumulate lp:{{
-  solve [int N] [goal _Ctx Ev Goal _Who] _OutGoals :-
-    coq.say "Goal:" {coq.term->string Goal},
-    check (qgen (qheight N)) (go Goal Term),
-    Ev = Term,
-    coq.say "Proof:" {coq.term->string Ev}.
- solve [str "size", int N] [goal _Ctx Ev Goal _Who] _OutGoals :-
-    coq.say "Goal:" {coq.term->string Goal},
-    check (qgen (qsize N M_)) (go Goal Term),
-    Ev = Term,
-    coq.say "Proof:" {coq.term->string Ev}.
-solve [str "pair", int H, int S ] [goal _Ctx Ev Goal _Who] _OutGoals :-
-      coq.say "Goal:" {coq.term->string Goal},
-    check (pair (qgen (qheight H)) (qgen (qsize S S2_ ))) (go Goal Term),
-    Ev = Term,
-    coq.say "Proof:" {coq.term->string Ev}.
-  }}.
- Elpi Typecheck. 
 
+ Elpi Query interp {{lp:G = lp:G}}.
  Elpi Bound Steps 1000000.
 
 Inductive insert (x:nat) : list nat -> list nat -> Prop :=
@@ -61,50 +42,3 @@ i_n : insert x [] [x]
 Goal insert 1 [] [1].
 elpi dprolog 10.
 Qed.
-Lemma i1:  exists R, insert 2 [0;1] R.
-elpi  dprolog 10.
-Qed.
-Lemma i2:  exists R, insert 2 [0;1] R.
-eexists.
-apply i_c.
-apply i_c.
-apply i_n.
-Qed.
-Print i2.
-Print le.
- Inductive ordered : list nat -> Prop :=
-onl : ordered []
-| oss : forall x : nat, ordered [x]
-| ocn : forall (x y : nat) (l : list nat),
-     ordered (y :: l) -> x <= y -> ordered (x :: y :: l).
-
-Goal exists Xs, ordered Xs.
-eexists.
-elpi prolog  3.
-apply onl.
-Restart.
-eexists.
-elpi dprolog 10.
-Qed.
-
- Goal ordered [0;1;2;6].
-   elpi prolog  10.
-   Fail elpi prolog size 10.
-
-   elpi dprolog 20.
-   Qed.
-
-   Inductive append : list nat -> list nat -> list nat -> Prop :=
-   anl : forall xs, append [] xs xs
-   |acn : forall xs ys zs x, 
-        append xs ys zs -> append (x :: xs) ys (x :: zs).
-
-  (* Goal exists L1 L2, append L1 L2 [0;1;2;6]. *)
-  Goal append  [0] [1;2;6] [0;1;2;6].
-  elpi dprolog 20.
-Qed.
-
- Goal exists L, append  L [1;2;6] [0;1;2;6].
- eexists.
- elpi dprolog  20.
- Qed.
