tactics/dprolog.v
@@ -1,0 +1,82 @@
+(* DEPENDENT "prolog"-like tactic modulo FPC for height, size and pairing thereof  -- am*)
+
+From elpi Require Import elpi.
+Require Import Arith List. Import ListNotations.
+Require Import Coq.Lists.List.
+
+
+Elpi Tactic dprolog.
+Elpi Accumulate File "pbt/dep-kernel.mod".
+Elpi Accumulate File "pbt/fpc-qbound.mod".
+Elpi Accumulate File "pbt/fpc-pair.mod".
+
+Elpi Accumulate lp:{{
+  solve [int N] [goal _Ctx Ev Goal _Who] _OutGoals :-
+    coq.say "Goal:" {coq.term->string Goal},
+    check (qgen (qheight N)) (go Goal Term),
+    Ev = Term,
+    coq.say "Proof:" {coq.term->string Ev}.
+ solve [str "size", int N] [goal _Ctx Ev Goal _Who] _OutGoals :-
+    coq.say "Goal:" {coq.term->string Goal},
+    check (qgen (qsize N M_)) (go Goal Term),
+    Ev = Term,
+    coq.say "Proof:" {coq.term->string Ev}.
+solve [str "pair", int H, int S ] [goal _Ctx Ev Goal _Who] _OutGoals :-
+      coq.say "Goal:" {coq.term->string Goal},
+    check (pair (qgen (qheight H)) (qgen (qsize S S2_ ))) (go Goal Term),
+    Ev = Term,
+    coq.say "Proof:" {coq.term->string Ev}.
+  }}.
+ Elpi Typecheck. 
+
+ Elpi Bound Steps 1000000.
+
+Inductive insert (x:nat) : list nat -> list nat -> Prop :=
+i_n : insert x [] [x]
+| i_s : forall y: nat, forall ys: list nat, x <= y -> insert x (y :: ys) (x :: y :: ys)
+| i_c : forall y: nat, forall ys: list nat, forall rs: list nat,  insert x ys rs -> insert x (y :: ys) (y :: rs).
+
+Goal insert 1 [] [1].
+elpi dprolog 10.
+Qed.
+Lemma i1:  exists R, insert 2 [0;1] R.
+elpi  dprolog 10.
+Qed.
+Lemma i2:  exists R, insert 2 [0;1] R.
+eexists.
+apply i_c.
+apply i_c.
+apply i_n.
+Qed.
+Print i2.
+Print le.
+ Inductive ordered : list nat -> Prop :=
+onl : ordered []
+| oss : forall x : nat, ordered [x]
+| ocn : forall (x y : nat) (l : list nat),
+     ordered (y :: l) -> x <= y -> ordered (x :: y :: l).
+
+Goal exists Xs, ordered Xs.
+eexists.
+elpi dprolog 10.
+Qed.
+
+ Goal ordered [0;1;2;6].
+   
+   elpi dprolog 20.
+   Qed.
+
+   Inductive append : list nat -> list nat -> list nat -> Prop :=
+   anl : forall xs, append [] xs xs
+   |acn : forall xs ys zs x, 
+        append xs ys zs -> append (x :: xs) ys (x :: zs).
+
+  (* Goal exists L1 L2, append L1 L2 [0;1;2;6]. *)
+  Goal append  [0] [1;2;6] [0;1;2;6].
+  elpi dprolog 20.
+Qed.
+
+ Goal exists L, append  L [1;2;6] [0;1;2;6].
+ eexists.
+ elpi dprolog  20.
+ Qed.
